src/tools/parallelcomposition/generaldeduction/sapic_comp_DY_sapicplusScript.sml
@@ -19,12 +19,12 @@ val _ = new_theory "sapic_comp_DY_sapicplus";
 
 val spaicplus_to_sapic_vs_DY_single_transition_thm = store_thm(
   "spaicplus_to_sapic_vs_DY_single_transition_thm",
-  ``∀e Re0 NRe0 i Re NRe Pr0 Pr (Sym:(Var_t -> bool)) (Sym':(Var_t -> bool)) (P:('SPpred + DYpred -> bool)) (P':('SPpred + DYpred -> bool)) (Ded:('SPpred) tded) (ded3:('SPpred + DYpred) tded).
-       sapic_plus_position_transition_with_symb (Sym,P,(Pconfig_plus (Pr0,0,Re0,NRe0))) e
-       (Sym',P',(Pconfig_plus (Pr,i,Re,NRe))) ⇒
+  ``∀e Re' NRe' i' i Re NRe Pr' Pr (Sym:(Var_t -> bool)) (Sym':(Var_t -> bool)) (P:('SPpred + DYpred -> bool)) (P':('SPpred + DYpred -> bool)) (Ded:('SPpred) tded) (ded3:('SPpred + DYpred) tded).
+       sapic_plus_position_transition_with_symb (Sym,P,(Pconfig_plus (Pr,i,Re,NRe))) e
+       (Sym',P',(Pconfig_plus (Pr',i',Re',NRe'))) ⇒
      ∃e1 e2.
-       sapic_position_transition_with_symb (Sym,IMAGE OUTL P,(Pconfig (Pr0,0,Re0,NRe0))) e1
-                                           (Sym',IMAGE OUTL P',(Pconfig (Pr,i,Re,NRe))) ∧
+       sapic_position_transition_with_symb (Sym,IMAGE OUTL P,(Pconfig (Pr,i,Re,NRe))) e1
+                                           (Sym',IMAGE OUTL P',(Pconfig (Pr',i',Re',NRe'))) ∧
        DYtranrel (Sym,IMAGE OUTR P,ESt) e2 (Sym',IMAGE OUTR P',ESt) ∧
        binterl [e1] [e2] [e]``,
 
@@ -103,7 +103,7 @@ val spaicplus_to_sapic_vs_DY_single_transition_thm = store_thm(
                 metis_tac[binterl_moveALN,binterl_nil]
                 ) >>
               FULL_SIMP_TAC (list_ss++pred_setSimps.PRED_SET_ss++boolSimps.LIFT_COND_ss++boolSimps.EQUIV_EXTRACT_ss)[FactTag_t_distinct,FactTag_t_case_def] >>
-              Cases_on ‘Pr0’ >- (
+              Cases_on ‘Pr’ >- (
                 FULL_SIMP_TAC (list_ss++pred_setSimps.PRED_SET_ss++boolSimps.LIFT_COND_ss++boolSimps.EQUIV_EXTRACT_ss)[Process_t_distinct,Process_t_case_def]
                 ) (*ProcessNull*) >- (
                 Cases_on ‘P2’ >- (
@@ -245,14 +245,14 @@ val spaicplus_to_sapic_vs_DY_single_transition_thm = store_thm(
 
 val sapic_vs_DY_to_spaicplus_single_transition_thm = store_thm(
   "sapic_vs_DY_to_spaicplus_single_transition_thm",
-  ``∀e Pr0 Pr Re0 NRe0 i Re NRe (Sym:(Var_t -> bool)) (Sym':(Var_t -> bool)) (P:('SPpred + DYpred -> bool)) (P':('SPpred + DYpred -> bool)) (Ded:('SPpred) tded) (ded3:('SPpred + DYpred) tded).
+  ``∀e Re' NRe' i' i Re NRe Pr' Pr (Sym:(Var_t -> bool)) (Sym':(Var_t -> bool)) (P:('SPpred + DYpred -> bool)) (P':('SPpred + DYpred -> bool)) (Ded:('SPpred) tded) (ded3:('SPpred + DYpred) tded).
        (∃e1 e2.
-          sapic_position_transition_with_symb (Sym,IMAGE OUTL P,(Pconfig (Pr0,0,Re0,NRe0))) e1
-                                              (Sym',IMAGE OUTL P',(Pconfig (Pr,i,Re,NRe))) ∧
+          sapic_position_transition_with_symb (Sym,IMAGE OUTL P,(Pconfig (Pr,i,Re,NRe))) e1
+                                              (Sym',IMAGE OUTL P',(Pconfig (Pr',i',Re',NRe'))) ∧
           DYtranrel (Sym,IMAGE OUTR P,ESt) e2 (Sym',IMAGE OUTR P',ESt) ∧
           binterl [e1] [e2] [e]) ⇒
-     (sapic_plus_position_transition_with_symb (Sym,P,(Pconfig_plus (Pr0,0,Re0,NRe0))) e
-      (Sym',P',(Pconfig_plus (Pr,i,Re,NRe)))) 
+     (sapic_plus_position_transition_with_symb (Sym,P,(Pconfig_plus (Pr,i,Re,NRe))) e
+      (Sym',P',(Pconfig_plus (Pr',i',Re',NRe')))) 
      ``,
      GEN_TAC >>
      Induct_on `e` >-
@@ -273,7 +273,7 @@ val sapic_vs_DY_to_spaicplus_single_transition_thm = store_thm(
         IMP_RES_TAC binterl_moveNAL >>
         rw[] >>
         IMP_RES_TAC sapic_position_transition_with_symb_def >>
-        Cases_on ‘Pr0’ >- (
+        Cases_on ‘Pr’ >- (
           IMP_RES_TAC sapic_position_transition_def >>
           FULL_SIMP_TAC (list_ss++pred_setSimps.PRED_SET_ss++boolSimps.LIFT_COND_ss++boolSimps.EQUIV_EXTRACT_ss)[Process_t_distinct,Process_t_case_def]
           )(*ProcessNull*) >-(
@@ -418,67 +418,56 @@ val sapic_vs_DY_to_spaicplus_single_transition_thm = store_thm(
       >> metis_tac[sapic_position_transition_with_symb_def]
       (*Alias*)              
       )(*end of 1-Case of (SOME (INR y)) *) >>
-      Cases_on ‘y'’  >- (
-        rpt strip_tac >>
-        IMP_RES_TAC binterl_moveSR >>
-        rw[] >>
-        IMP_RES_TAC sapic_position_transition_with_symb_def >>
-        IMP_RES_TAC DYtranrel_def >>
-        rw[sapic_plus_position_transition_with_symb_def]
-        )(*end of 1-Case of (SOME (INR (INR y))) => P2A *) >- (
-        rpt strip_tac >>
-        IMP_RES_TAC binterl_moveSR >>
-        rw[] >>
-        IMP_RES_TAC sapic_position_transition_with_symb_def >>
-        IMP_RES_TAC DYtranrel_def >>
-        rw[sapic_plus_position_transition_with_symb_def]
-        )(*A2P*) >>
+     Cases_on ‘y'’  >- (
       rpt strip_tac >>
       IMP_RES_TAC binterl_moveSR >>
       rw[] >>
       IMP_RES_TAC sapic_position_transition_with_symb_def >>
       IMP_RES_TAC DYtranrel_def >>
       rw[sapic_plus_position_transition_with_symb_def]
+      )(*end of 1-Case of (SOME (INR (INR y))) => P2A *) >- (
+      rpt strip_tac >>
+      IMP_RES_TAC binterl_moveSR >>
+      rw[] >>
+      IMP_RES_TAC sapic_position_transition_with_symb_def >>
+      IMP_RES_TAC DYtranrel_def >>
+      rw[sapic_plus_position_transition_with_symb_def]
+      )(*A2P*) >>
+     rpt strip_tac >>
+     IMP_RES_TAC binterl_moveSR >>
+     rw[] >>
+     IMP_RES_TAC sapic_position_transition_with_symb_def >>
+     IMP_RES_TAC DYtranrel_def >>
+     rw[sapic_plus_position_transition_with_symb_def]
   )(*end of theorem*)      
 
-             
 
+val sapic_vs_DY_EQ_spaicplus_single_transition_thm = store_thm(
+  "sapic_vs_DY_EQ_spaicplus_single_transition_thm",
+  ``∀e Re' NRe' i' i Re NRe Pr' Pr (Sym:(Var_t -> bool)) (Sym':(Var_t -> bool)) (P:('SPpred + DYpred -> bool)) (P':('SPpred + DYpred -> bool)) (Ded:('SPpred) tded) (ded3:('SPpred + DYpred) tded).
+       (∃e1 e2.
+          sapic_position_transition_with_symb (Sym,IMAGE OUTL P,(Pconfig (Pr,i,Re,NRe))) e1
+                                              (Sym',IMAGE OUTL P',(Pconfig (Pr',i',Re',NRe'))) ∧
+          DYtranrel (Sym,IMAGE OUTR P,ESt) e2 (Sym',IMAGE OUTR P',ESt) ∧
+          binterl [e1] [e2] [e]) =
+     (sapic_plus_position_transition_with_symb (Sym,P,(Pconfig_plus (Pr,i,Re,NRe))) e
+      (Sym',P',(Pconfig_plus (Pr',i',Re',NRe')))) 
+     ``,
+     rpt gen_tac >>
+     EQ_TAC >>
+     rewrite_tac[sapic_vs_DY_to_spaicplus_single_transition_thm] >>
+     rewrite_tac[spaicplus_to_sapic_vs_DY_single_transition_thm]
+  )
+                                                              
 
-
-
-
-
-
-
-
-
-
-
-
-
-
-
-     (*                                                            
-                       
-rw[sapic_plus_position_transition_with_symb_def,sapic_plus_position_transition_def]            Cases_on `l` >- (        
-                  FULL_SIMP_TAC (list_ss++pred_setSimps.PRED_SET_ss++boolSimps.LIFT_COND_ss++boolSimps.EQUIV_EXTRACT_ss)[]) >>
-                  FULL_SIMP_TAC (list_ss++pred_setSimps.PRED_SET_ss++boolSimps.LIFT_COND_ss++boolSimps.EQUIV_EXTRACT_ss)[] >>
-reverse (Cases_on `t`) >- (        
-                FULL_SIMP_TAC (list_ss++pred_setSimps.PRED_SET_ss++boolSimps.LIFT_COND_ss++boolSimps.EQUIV_EXTRACT_ss)[]) >- (        
-                  FULL_SIMP_TAC (list_ss++pred_setSimps.PRED_SET_ss++boolSimps.LIFT_COND_ss++boolSimps.EQUIV_EXTRACT_ss)[] >>
-
-                  )                              
-                
-
-        
-val spaicplus_to_sapic_vs_DY_thm = store_thm(
-  "spaicplus_to_sapic_vs_DY_thm",
+val spaicplus_to_sapic_vs_DY_multi_transitions_thm = store_thm(
+  "spaicplus_to_sapic_vs_DY_multi_transitions_thm",
   ``∀t Re0 NRe0 i Re NRe Pr0 Pr (Sym:(Var_t -> bool)) (Sym':(Var_t -> bool)) (P:('SPpred + DYpred -> bool)) (P':('SPpred + DYpred -> bool)) (Ded:('SPpred) tded) (ded3:('SPpred + DYpred) tded).
        sapic_plus_position_multi_transitions_with_symb (Sym,P,(Pconfig_plus (Pr0,0,Re0,NRe0))) t
        (Sym',P',(Pconfig_plus (Pr,i,Re,NRe))) ⇒
      ∃t1 t2.
        sapic_position_multi_transitions_with_symb (Sym,IMAGE OUTL P,(Pconfig (Pr0,0,Re0,NRe0))) t1
-       (Sym',IMAGE OUTL P',(Pconfig (Pr,i,Re,NRe))) ∧
+                                                  (Sym',IMAGE OUTL P',(Pconfig (Pr,i,Re,NRe))) ∧
        DYmultranrel (Sym,IMAGE OUTR P,ESt) t2 (Sym',IMAGE OUTR P',ESt) ∧
        binterl t1 t2 t``,
                GEN_TAC >>
@@ -488,90 +477,90 @@ val spaicplus_to_sapic_vs_DY_thm = store_thm(
       Q.EXISTS_TAC `[]` >>
       Q.EXISTS_TAC `[]` >>
       rw[binterl_nil,TranRelConfigEq,DYmultranrel_def] >>
-      metis_tac[sapic_position_multi_transitions_with_symb_nil]) >>
-     Cases_on `h` >- (
-      rpt strip_tac >>
-      IMP_RES_TAC TranRelSnocRev >>
-      PAT_X_ASSUM ``!Re0 NRe0 i Re NRe Pr0 Pr Sym Sym' P P'. A`` (ASSUME_TAC o (Q.SPECL [`Re0`,`NRe0`,`i`,`Re`,`NRe`,`Pr0`,`Pr`,`Sym`,`Sym'`,`P`,`P'`]))>>
-      PAT_X_ASSUM ``!v' s' p'. A`` (ASSUME_TAC o (Q.SPECL [`Sym'`,`(Pconfig_plus (Pr,i,Re,NRe))`,`P'`])) >>
-      PAT_X_ASSUM ``!v' s' p'. A`` (ASSUME_TAC o (Q.SPECL [`Sym'`,`(Pconfig_plus (Pr,i,Re,NRe))`,`P'`])) >>
-      RES_TAC >>
-      Q.EXISTS_TAC `t1` >>
-      Q.EXISTS_TAC `t2` >>
-      metis_tac[binterl_combinenone] 
+      metis_tac[sapic_position_multi_transitions_with_symb_nil]
       ) >>
-     Cases_on `x` >-(
-      Cases_on `x'` >-(
-        rpt strip_tac >>
-        IMP_RES_TAC TranRelSnocRev >>
-        PAT_X_ASSUM ``!Re0 NRe0 i Re NRe Pr0 Pr Sym Sym' P P' Ded ded3. A`` (ASSUME_TAC o (Q.SPECL [`Re0`,`NRe0`,`i''`,`Re''`,`NRe''`,`Pr0`,`Pr''`,`Sym`,`Sym''`,`P`,`P''`,`Ded`,`ded3`]))>>
-      PAT_X_ASSUM ``!v' s' p'. A`` (ASSUME_TAC o (Q.SPECL [`Sym''`,`(Pconfig_plus (Pr'',i'',Re'',NRe''))`,`P''`])) >>
-        PAT_X_ASSUM ``!v' s' p'. A`` (ASSUME_TAC o (Q.SPECL [`Sym''`,`(Pconfig_plus (Pr'',i'',Re'',NRe''))`,`P''`]))>>
-        RES_TAC >>
-        Q.EXISTS_TAC `(SOME (INL x))::t1` >>
-        Q.EXISTS_TAC `t2` >>
-        reverse (rw[binterl_left])
-                
-        metis_tac[TranRelNil,TranRelSnoc,TranRelConfigEq,sapic_position_multi_transitions_with_symb_move]
-        ) >>
+     rpt strip_tac >>
+     IMP_RES_TAC TranRelSnocRev >>
+     PAT_X_ASSUM ``!v' s' p'. A`` (ASSUME_TAC o (Q.SPECL [`Sym''`,`(Pconfig_plus (Pr'',i'',Re'',NRe''))`,`P''`])) >>
+     PAT_X_ASSUM ``!v' s' p'. A`` (ASSUME_TAC o (Q.SPECL [`Sym''`,`(Pconfig_plus (Pr'',i'',Re'',NRe''))`,`P''`])) >>                     
+     PAT_X_ASSUM ``!Re0 NRe0 i Re NRe Pr0 Pr Sym Sym' P P' Ded ded3. A`` (ASSUME_TAC o (Q.SPECL [`Re0`,`NRe0`,`i''`,`Re''`,`NRe''`,`Pr0`,`Pr''`,`Sym`,`Sym''`,`P`,`P''`,`Ded`,`ded3`]))>>
+     RES_TAC >>
+     IMP_RES_TAC sapic_plus_position_with_symb_single >>
+     IMP_RES_TAC spaicplus_to_sapic_vs_DY_single_transition_thm >>             
+     Q.EXISTS_TAC `e1::t1` >>
+     Q.EXISTS_TAC `e2::t2` >>
+     metis_tac[sapic_position_multi_transitions_with_symb_moveF,DYmultranrel_move,binterl_moveF]
+  )
 
 
-                        
-FULL_SIMP_TAC (list_ss++pred_setSimps.PRED_SET_ss++boolSimps.LIFT_COND_ss++boolSimps.EQUIV_EXTRACT_ss)[]
-FULL_SIMP_TAC (list_ss++pred_setSimps.PRED_SET_ss++boolSimps.LIFT_COND_ss++boolSimps.EQUIV_EXTRACT_ss)[sapic_position_multi_transitions_with_symb_move] >>
-sapic_position_transition_def
+val sapic_vs_DY_to_spaicplus_multi_transitions_thm = store_thm(
+  "sapic_vs_DY_to_spaicplus_multi_transitions_thm",
+  ``∀t Re0 NRe0 i Re NRe Pr0 Pr (Sym:(Var_t -> bool)) (Sym':(Var_t -> bool)) (P:('SPpred + DYpred -> bool)) (P':('SPpred + DYpred -> bool)) (Ded:('SPpred) tded) (ded3:('SPpred + DYpred) tded).
+       (∃t1 t2.
+          sapic_position_multi_transitions_with_symb (Sym,IMAGE OUTL P,(Pconfig (Pr0,0,Re0,NRe0))) t1
+                                                     (Sym',IMAGE OUTL P',(Pconfig (Pr,i,Re,NRe))) ∧
+          DYmultranrel (Sym,IMAGE OUTR P,ESt) t2 (Sym',IMAGE OUTR P',ESt) ∧
+          binterl t1 t2 t) ⇒
+     (sapic_plus_position_multi_transitions_with_symb (Sym,P,(Pconfig_plus (Pr0,0,Re0,NRe0))) t
+      (Sym',P',(Pconfig_plus (Pr,i,Re,NRe))))
+     ``,
+     GEN_TAC >>
+     Induct_on `t` >- (
+      rpt strip_tac >>
+      IMP_RES_TAC binterl_Empty >>
+      rw[] >>
+      IMP_RES_TAC TranRelConfigEq >>
+      rw[]>>
+      metis_tac[sapic_plus_position_multi_transitions_with_symb_nil,IMAGEOUT]
+      ) >>
+     rpt strip_tac >>
+     IMP_RES_TAC binterl_NotEmpty >>
+     rw[] >>
+     IMP_RES_TAC TranRelSnocBack >>
+     PAT_X_ASSUM ``!v' s' p'. A`` (ASSUME_TAC o (Q.SPECL [`Sym''`,`ESt`,`IMAGE OUTR (P'':('SPpred + DYpred -> bool))`])) >>
+     PAT_X_ASSUM ``!v' s' p'. A`` (ASSUME_TAC o (Q.SPECL [`Sym''`,`ESt`,`IMAGE OUTR (P'':('SPpred + DYpred -> bool))`])) >>
+     PAT_X_ASSUM ``!v' s' p'. A`` (ASSUME_TAC o (Q.SPECL [`Sym''`,`(Pconfig (Pr'',i'',Re'',NRe''))`,`IMAGE OUTL (P'':('SPpred + DYpred -> bool))`])) >>
+     PAT_X_ASSUM ``!v' s' p'. A`` (ASSUME_TAC o (Q.SPECL [`Sym''`,`(Pconfig (Pr'',i'',Re'',NRe''))`,`IMAGE OUTL (P'':('SPpred + DYpred -> bool))`])) >>
+     IMP_RES_TAC binterl_Conj >>
+     PAT_X_ASSUM ``!Re0 NRe0 i Re NRe Pr0 Pr Sym Sym' P P' Ded ded3. A`` (ASSUME_TAC o (Q.SPECL [`Re0`,`NRe0`,`i''`,`Re''`,`NRe''`,`Pr0`,`Pr''`,`Sym`,`Sym''`,`P`,`P''`,`Ded`,`ded3`]))>>          RES_TAC  >>
+     IMP_RES_TAC DYmultranrel_single >>
+     IMP_RES_TAC sapic_position_with_symb_single >>
+     IMP_RES_TAC sapic_vs_DY_to_spaicplus_single_transition_thm >> 
+     IMP_RES_TAC sapic_plus_position_with_symb_single >>
+     metis_tac[sapic_plus_position_multi_transitions_with_symb_moveF]
+  )
 
 
-                         
-val SapRelConfigEq = new_axiom ("SapRelConfigEq",
-                            ``∀Pr i Re NRe i Pr' i' Re' NRe'. (sapic_plus_position_multi_transitions (Pconfig_plus (Pr,i,Re,NRe)) [] (Pconfig_plus (Pr',i',Re',NRe'))) ⇒ ((Pr = Pr')∧(i = i')∧(Re = Re')∧(NRe = NRe'))``);
-             
-val compose_sapic_vs_DY_spaicplus_thm = store_thm(
-  "compose_sapic_vs_DY_spaicplus_thm",
+val sapic_vs_DY_EQ_spaicplus_multi_transitions_thm = store_thm(
+  "sapic_vs_DY_EQ_spaicplus_multi_transitions_thm",
+  ``∀t Re0 NRe0 i Re NRe Pr0 Pr (Sym:(Var_t -> bool)) (Sym':(Var_t -> bool)) (P:('SPpred + DYpred -> bool)) (P':('SPpred + DYpred -> bool)) (Ded:('SPpred) tded) (ded3:('SPpred + DYpred) tded).
+       (∃t1 t2.
+          sapic_position_multi_transitions_with_symb (Sym,IMAGE OUTL P,(Pconfig (Pr0,0,Re0,NRe0))) t1
+                                                     (Sym',IMAGE OUTL P',(Pconfig (Pr,i,Re,NRe))) ∧
+          DYmultranrel (Sym,IMAGE OUTR P,ESt) t2 (Sym',IMAGE OUTR P',ESt) ∧
+          binterl t1 t2 t) =
+     (sapic_plus_position_multi_transitions_with_symb (Sym,P,(Pconfig_plus (Pr0,0,Re0,NRe0))) t
+      (Sym',P',(Pconfig_plus (Pr,i,Re,NRe)))) 
+     ``,
+     rpt strip_tac>>
+     EQ_TAC>>
+     rewrite_tac[sapic_vs_DY_to_spaicplus_multi_transitions_thm] >>
+     rewrite_tac[spaicplus_to_sapic_vs_DY_multi_transitions_thm] 
+  )
+
+
+val comptraces_sapic_vs_DY_EQ_sapic_plus_traces_thm = store_thm(
+  "comptraces_sapic_vs_DY_EQ_sapic_plus_traces_thm",
   ``∀t Re0 NRe0 i Re NRe Pr0 Pr (Sym:(Var_t -> bool)) (Sym':(Var_t -> bool)) (P:('SPpred + DYpred -> bool)) (P':('SPpred + DYpred -> bool)) (Ded:('SPpred) tded) (ded3:('SPpred + DYpred) tded).
        (comptraces (sapic_position_multi_transitions_with_symb,Ded) (DYmultranrel,DYdeduction) ded3 (Sym,P,(Pconfig (Pr0,0,Re0,NRe0)),ESt) (Sym',P',(Pconfig (Pr,i,Re,NRe)),ESt)) =
      (sapic_plus_traces sapic_plus_position_multi_transitions_with_symb (Sym,P,(Pconfig_plus (Pr0,0,Re0,NRe0))) (Sym',P',(Pconfig_plus (Pr,i,Re,NRe))))``,
-     rewrite_tac[binterleave_composition_generaldeduction,binterleave_ts]>>
+                                                                                                                                                       rewrite_tac[binterleave_composition_generaldeduction,binterleave_ts]>>
      rewrite_tac[sapic_plus_traces_def]>>
      rewrite_tac[traces_def]>>
      FULL_SIMP_TAC (list_ss++pred_setSimps.PRED_SET_ss++boolSimps.LIFT_COND_ss++boolSimps.EQUIV_EXTRACT_ss) [EXTENSION]>>
-     rpt strip_tac>>
-     EQ_TAC>>
-     Induct_on `x` >-
-      (rpt strip_tac >>
-       IMP_RES_TAC binterl_Empty >>
-       rw[]>>
-       IMP_RES_TAC TranRelConfigEq >>
-       rw[]>>
-       metis_tac[sapic_plus_position_multi_transitions_with_symb_nil,IMAGEOUT]) >>
-gen_tac >>
-     reverse(Cases_on `h`) >-
-      (Cases_on `x'` >- (
-        Cases_on `x''` >- 
-         (
-          rpt strip_tac >>
-          IMP_RES_TAC binterl_moveAL >>
-          rw[] >>
-          IMP_RES_TAC TranRelSnocRevAsyncL >>
-          Q.EXISTS_TAC `Sym''` >>
-          Q.EXISTS_TAC `P''` >>
-          Q.EXISTS_TAC `S1''` >>
-          rw[]
-          >- (metis_tac[sapic_plus_position_multi_transitions_with_symb_move,IMAGEOUT]) >>
-          PAT_X_ASSUM ``!Sym P S1 S2 Sym' P' S1' S2' MTrn1 MTrn2 ded1 ded2 ded3. A`` (ASSUME_TAC o (Q.SPECL [`Sym`,`P`,`S1`,`S2`,`Sym''`,`P''`,`S1''`,`S2'`,`MTrn1`,`MTrn2`,`ded1`,`ded2`,`ded3`])) >>
-          IMP_RES_TAC binterl_movesL >>
-          RES_TAC)
-
-        
-rewrite_tac[comptraces_def]
-rewrite_tac[sapic_plus_traces_def]
-FULL_SIMP_TAC (list_ss++pred_setSimps.PRED_SET_ss++boolSimps.LIFT_COND_ss++boolSimps.EQUIV_EXTRACT_ss) [EXTENSION]EQ_TAC                                                                                                                                                                                                                                                                        
-rewrite_tac[binterleave_composition_generaldeduction,binterleave_ts,symbtree_to_sapic_trace_inclusion_thm] >>
-FULL_SIMP_TAC (list_ss++pred_setSimps.PRED_SET_ss++boolSimps.LIFT_COND_ss++boolSimps.EQUIV_EXTRACT_ss) [SUBSET_DEF] >>
-     metis_tac[]
-              );
+     rewrite_tac[sapic_vs_DY_EQ_spaicplus_multi_transitions_thm]
+  )                       
 
 
-*)
 
 val _ = export_theory();
